Working on paranoid sanity.

formalization/ptt.v
@@ -36,8 +36,34 @@ with issubst : substitution -> context -> context -> Type :=
            isctx D ->
            issubst sbs G D ->
            istype D A ->
-           issubst (sbshift G A sbs) (ctxextend G (Subst A sbs)) (ctxextend D A)
+           issubst (sbshift G A sbs)
+                   (ctxextend G (Subst A sbs))
+                   (ctxextend D A)
 
+     | SubstId :
+         forall {G},
+           isctx G ->
+           issubst (sbid G) G G
+
+     | SubstComp :
+         forall {G D E sbs sbt},
+           isctx G ->
+           isctx D ->
+           isctx E ->
+           issubst sbs G D ->
+           issubst sbt D E ->
+           issubst (sbcomp sbt sbs) G E
+
+     | SubstCtxConv :
+         forall {G1 G2 D1 D2 sbs},
+           isctx G1 ->
+           isctx G2 ->
+           isctx D1 ->
+           isctx D2 ->
+           issubst sbs G1 D1 ->
+           eqctx G1 G2 ->
+           eqctx D1 D2 ->
+           issubst sbs G2 D2
 
 
 with istype : context -> type -> Type :=
@@ -95,8 +121,8 @@ with isterm : context -> term -> type -> Type :=
      | TermTyConv :
          forall {G A B u},
            isctx G ->
-           istype A ->
-           istype B ->
+           istype G A ->
+           istype G B ->
            isterm G u A ->
            eqtype G A B ->
            isterm G u B
@@ -246,6 +272,28 @@ with isterm : context -> term -> type -> Type :=
 
 with eqctx : context -> context -> Type :=
 
+
+     | CtxRefl :
+         forall {G},
+           isctx G ->
+           eqctx G G
+
+     | CtxSym :
+         forall {G D},
+           isctx G ->
+           isctx D ->
+           eqctx G D ->
+           eqctx D G
+
+     | CtxTrans :
+         forall {G D E},
+           isctx G ->
+           isctx D ->
+           isctx E ->
+           eqctx G D ->
+           eqctx D E ->
+           eqctx G E
+
      | EqCtxEmpty :
          eqctx ctxempty ctxempty
 
@@ -257,6 +305,189 @@ with eqctx : context -> context -> Type :=
            eqtype G A B ->
            eqctx (ctxextend G A) (ctxextend G B)
 
+
+with eqsubst : substitution -> substitution -> context -> context -> Type :=
+
+     | SubstRefl :
+         forall {G D sbs},
+           isctx G ->
+           isctx D ->
+           issubst sbs G D ->
+           eqsubst sbs sbs G D
+
+     | SubstSym :
+         forall {G D sbs sbt},
+           isctx G ->
+           isctx D ->
+           issubst sbs G D ->
+           issubst sbt G D ->
+           eqsubst sbs sbt G D ->
+           eqsubst sbt sbs G D
+
+     | SubstTrans :
+         forall {G D sb1 sb2 sb3},
+           isctx G ->
+           isctx D ->
+           issubst sb1 G D ->
+           issubst sb2 G D ->
+           issubst sb3 G D ->
+           eqsubst sb1 sb2 G D ->
+           eqsubst sb2 sb3 G D ->
+           eqsubst sb1 sb3 G D
+
+     | CongSubstZero :
+         forall {G1 G2 A1 A2 u1 u2},
+           isctx G1 ->
+           isctx G2 ->
+           istype G1 A1 ->
+           istype G1 A2 ->
+           isterm G1 u1 A1 ->
+           isterm G1 u2 A1 ->
+           eqctx G1 G2 ->
+           eqtype G1 A1 A2 ->
+           eqterm G1 u1 u2 A1 ->
+           eqsubst (sbzero G1 A1 u1)
+                   (sbzero G1 A2 u2)
+                   G1
+                   (ctxextend G1 A1)
+
+     | CongSubstWeak :
+         forall {G1 G2 A1 A2},
+           isctx G1 ->
+           isctx G2 ->
+           istype G1 A1 ->
+           istype G1 A2 ->
+           eqctx G1 G2 ->
+           eqtype G1 A1 A2 ->
+           eqsubst (sbweak G1 A1)
+                   (sbweak G2 A2)
+                   (ctxextend G1 A1)
+                   G1
+
+     | CongSubstShift :
+         forall {G1 G2 D A1 A2 sbs1 sbs2},
+           isctx G1 ->
+           isctx G2 ->
+           isctx D ->
+           istype G1 A1 ->
+           istype G1 A2 ->
+           issubst sbs1 G1 D ->
+           issubst sbs2 G1 D ->
+           eqctx G1 G2 ->
+           eqsubst sbs1 sbs2 G1 D ->
+           eqtype D A1 A2 ->
+           eqsubst (sbshift G1 A1 sbs1)
+                   (sbshift G2 A2 sbs2)
+                   (ctxextend G1 (Subst A1 sbs1))
+                   (ctxextend D A1)
+
+     | CongSubstComp :
+         forall {G D E sbs1 sbs2 sbt1 sbt2},
+           isctx G ->
+           isctx D ->
+           isctx E ->
+           issubst sbs1 G D ->
+           issubst sbs2 G D ->
+           issubst sbt1 D E ->
+           issubst sbt2 D E ->
+           eqsubst sbs1 sbs2 G D ->
+           eqsubst sbt1 sbt2 D E ->
+           eqsubst (sbcomp sbt1 sbs1)
+                   (sbcomp sbt2 sbs2)
+                   G
+                   E
+
+     | EqSubstCtxConv :
+         forall {G1 G2 D1 D2 sbs sbt},
+           isctx G1 ->
+           isctx G2 ->
+           isctx D1 ->
+           isctx D2 ->
+           issubst sbs G1 D1 ->
+           issubst sbt G1 D1 ->
+           eqsubst sbs sbt G1 D1 ->
+           eqctx G1 G2 ->
+           eqctx D1 D2 ->
+           eqsubst sbs sbt G2 D2
+
+     | CompAssoc :
+         forall {G D E F sbs sbt sbr},
+           isctx G ->
+           isctx D ->
+           isctx E ->
+           isctx F ->
+           issubst sbs G D ->
+           issubst sbt D E ->
+           issubst sbr E F ->
+           eqsubst (sbcomp (sbcomp sbr sbt) sbs)
+                   (sbcomp sbr (sbcomp sbt sbs))
+                   G
+                   F
+
+     | WeakNat :
+         forall {G D A sbs},
+           isctx G ->
+           isctx D ->
+           issubst sbs G D ->
+           istype D A ->
+           eqsubst (sbcomp (sbweak D A)
+                           (sbshift G A sbs))
+                   (sbcomp sbs
+                           (sbweak G (Subst A sbs)))
+                   (ctxextend G (Subst A sbs))
+                   D
+
+     | WeakZero :
+         forall {G A u},
+           isctx G ->
+           istype G A ->
+           isterm G u A ->
+           eqsubst (sbcomp (sbweak G A) (sbzero G A u))
+                   (sbid G)
+                   G
+                   G
+
+     | ShiftZero :
+         forall {G D A u sbs},
+           isctx G ->
+           isctx D ->
+           istype D A ->
+           issubst sbs G D ->
+           isterm D u A ->
+           eqsubst (sbcomp (sbshift G A sbs)
+                           (sbzero G (Subst A sbs) (subst u sbs)))
+                   (sbcomp (sbzero D A u)
+                           sbs)
+                   G
+                   (ctxextend D A)
+
+     | CompShift :
+         forall {G D E A sbs sbt},
+           isctx G ->
+           isctx D ->
+           isctx E ->
+           issubst sbs G D ->
+           issubst sbt D E ->
+           istype E A ->
+           eqsubst (sbcomp (sbshift D A sbt)
+                           (sbshift G (Subst A sbt) sbs))
+                   (sbshift G A (sbcomp sbt sbs))
+                   (ctxextend G (Subst A (sbcomp sbt sbs)))
+                   (ctxextend E A)
+
+     | CompIdRight :
+         forall {G D sbs},
+           isctx G ->
+           isctx D ->
+           issubst sbs G D ->
+           eqsubst (sbcomp (sbid D) sbs) sbs G D
+
+     | CompIdLeft :
+         forall {G D sbs},
+           isctx G ->
+           isctx D ->
+           issubst sbs G D ->
+           eqsubst (sbcomp sbs (sbid G)) sbs G D
 
 
 with eqtype : context -> type -> type -> Type :=
@@ -295,53 +526,31 @@ with eqtype : context -> type -> type -> Type :=
            eqtype G B C ->
            eqtype G A C
 
-     | EqTyWeakNat :
-         forall {G D A B sbs},
-           isctx G ->
-           isctx D ->
-           issubst sbs G D ->
-           istype D A ->
-           istype D B ->
-           eqtype (ctxextend G (Subst A sbs))
-                  (Subst (Subst B (sbweak D A)) (sbshift G A sbs))
-                  (Subst (Subst B sbs) (sbweak G (Subst A sbs)))
-
-     | EqTyWeakZero :
-         forall {G A B u},
+     | EqTyIdSubst :
+         forall {G A},
            isctx G ->
            istype G A ->
-           istype G B ->
-           isterm G u B ->
-           eqtype G (Subst (Subst A (sbweak G B)) (sbzero G B u)) A
+           eqtype G
+                  (Subst A (sbid G))
+                  A
 
-     | EqTyShiftZero :
-         forall {G D A B v sbs},
+     | EqTySubstComp :
+         forall {G D E A sbs sbt},
            isctx G ->
            isctx D ->
-           istype G A ->
+           isctx E ->
+           istype E A ->
            issubst sbs G D ->
-           istype (ctxextend D A) B ->
-           isterm D v A ->
+           issubst sbt D E ->
            eqtype G
-                  (Subst (Subst B (sbshift G A sbs)) (sbzero G (Subst A sbs) (subst v sbs)))
-                  (Subst (Subst B (sbzero D A v)) sbs)
+                  (Subst (Subst A sbt) sbs)
+                  (Subst A (sbcomp sbt sbs))
 
-     | EqTyCongZero :
-         forall {G A1 A2 B1 B2 u1 u2},
-           isctx G ->
-           istype G A1 ->
-           istype G B1 ->
-           istype (ctxextend G A1) A2 ->
-           istype (ctxextend G A1) B2 ->
-           eqtype G A1 B1 ->
-           eqterm G u1 u2 A1 ->
-           eqtype (ctxextend G A1) A2 B2 ->
-           eqtype G
-                  (Subst A2 (sbzero G A1 u1))
-                  (Subst B2 (sbzero G B1 u2))
 
      | EqTySubstProd :
          forall {G D A B sbs},
+           isctx G ->
+           isctx D ->
            issubst sbs G D ->
            istype D A ->
            istype (ctxextend D A) B ->
@@ -351,6 +560,8 @@ with eqtype : context -> type -> type -> Type :=
 
      | EqTySubstId :
          forall {G D A u v sbs},
+           isctx G ->
+           isctx D ->
            issubst sbs G D ->
            istype D A ->
            isterm D u A ->
@@ -361,6 +572,8 @@ with eqtype : context -> type -> type -> Type :=
 
      | EqTySubstEmpty :
          forall {G D sbs},
+           isctx G ->
+           isctx D ->
            issubst sbs G D ->
            eqtype G
                   (Subst Empty sbs)
@@ -368,6 +581,8 @@ with eqtype : context -> type -> type -> Type :=
 
      | EqTySubstUnit :
          forall {G D sbs},
+           isctx G ->
+           isctx D ->
            issubst sbs G D ->
            eqtype G
                   (Subst Unit sbs)
@@ -375,6 +590,8 @@ with eqtype : context -> type -> type -> Type :=
 
      | EqTySubstBool :
          forall {G D sbs},
+           isctx G ->
+           isctx D ->
            issubst sbs G D ->
            eqtype G
                   (Subst Bool sbs)
@@ -382,6 +599,7 @@ with eqtype : context -> type -> type -> Type :=
 
      | EqTyExfalso :
          forall {G A B u},
+           isctx G ->
            istype G A ->
            istype G B ->
            isterm G u Empty ->
@@ -389,58 +607,121 @@ with eqtype : context -> type -> type -> Type :=
 
      | CongProd :
          forall {G A1 A2 B1 B2},
+           isctx G ->
+           istype G A1 ->
+           istype (ctxextend G A1) A2 ->
+           istype G B1 ->
+           istype (ctxextend G A1) B2 ->
            eqtype G A1 B1 ->
            eqtype (ctxextend G A1) A2 B2 ->
            eqtype G (Prod A1 A2) (Prod B1 B2)
 
      | CongId :
          forall {G A B u1 u2 v1 v2},
+           isctx G ->
+           istype G A ->
+           istype G B ->
+           isterm G u1 A ->
+           isterm G u2 A ->
+           isterm G v1 A ->
+           isterm G v2 A ->
            eqtype G A B ->
            eqterm G u1 v1 A ->
            eqterm G u2 v2 A ->
            eqtype G (Id A u1 u2) (Id B v1 v2)
 
      | CongTySubst :
-         forall {G D A B sbs},
+         forall {G D A B sbs sbt},
+           isctx G ->
+           isctx D ->
+           istype D A ->
+           istype D B ->
            issubst sbs G D ->
+           issubst sbt G D ->
            eqtype D A B ->
-           eqtype G (Subst A sbs) (Subst B sbs)
-
+           eqtype G (Subst A sbs) (Subst B sbt)
 
 
 with eqterm : context -> term -> term -> type -> Type :=
 
      | EqTyConv :
          forall {G A B u v},
+           isctx G ->
+           istype G A ->
+           istype G B ->
+           isterm G u A ->
+           isterm G v A ->
            eqterm G u v A ->
            eqtype G A B ->
            eqterm G u v B
 
      | EqCtxConv :
          forall {G D u v A},
+           isctx G ->
+           isctx D ->
+           istype G A ->
+           isterm G u A ->
+           isterm G v A ->
            eqterm G u v A ->
            eqctx G D ->
            eqterm D u v A
 
      | EqRefl :
          forall {G A u},
+           isctx G ->
+           istype G A ->
            isterm G u A ->
            eqterm G u u A
 
      | EqSym :
          forall {G A u v},
+           isctx G ->
+           istype G A ->
+           isterm G u A ->
+           isterm G v A ->
            eqterm G v u A ->
            eqterm G u v A
 
      | EqTrans :
          forall {G A u v w},
+           isctx G ->
+           istype G A ->
+           isterm G u A ->
+           isterm G v A ->
+           isterm G w A ->
            eqterm G u v A ->
            eqterm G v w A ->
            eqterm G u w A
 
 
+     | EqIdSubst :
+         forall {G A u},
+           isctx G ->
+           istype G A ->
+           isterm G u A ->
+           eqterm G
+                  (subst u (sbid G))
+                  u
+                  A
+
+     | EqSubstComp :
+         forall {G D E A u sbs sbt},
+           isctx G ->
+           isctx D ->
+           isctx E ->
+           istype E A ->
+           isterm E u A ->
+           issubst sbs G D ->
+           issubst sbt D E ->
+           eqterm G
+                  (subst (subst u sbt) sbs)
+                  (subst u (sbcomp sbt sbs))
+                  (Subst A (sbcomp sbt sbs))
+
      | EqSubstWeak :
          forall {G A B k},
+           isctx G ->
+           istype G A ->
            isterm G (var k) A ->
            istype G B ->
            eqterm (ctxextend G B)
@@ -451,6 +732,8 @@ with eqterm : context -> term -> term -> type -> Type :=
 
      | EqSubstZeroZero :
          forall {G u A},
+           isctx G ->
+           istype G A ->
            isterm G u A ->
            eqterm G
                   (subst (var 0) (sbzero G A u))
@@ -459,6 +742,9 @@ with eqterm : context -> term -> term -> type -> Type :=
 
      | EqSubstZeroSucc :
          forall {G A B u k},
+           isctx G ->
+           istype G A ->
+           istype G B ->
            isterm G (var k) A ->
            isterm G u B ->
            eqterm G
@@ -468,6 +754,8 @@ with eqterm : context -> term -> term -> type -> Type :=
 
      | EqSubstShiftZero :
          forall {G D A sbs},
+           isctx G ->
+           isctx D ->
            issubst sbs G D ->
            istype D A ->
            eqterm (ctxextend G (Subst A sbs))
@@ -477,6 +765,9 @@ with eqterm : context -> term -> term -> type -> Type :=
 
      | EqSubstShiftSucc :
          forall { G D A B sbs k },
+           isctx G ->
+           isctx D ->
+           istype D B ->
            issubst sbs G D ->
            isterm D (var k) B ->
            istype D A ->
@@ -487,9 +778,12 @@ with eqterm : context -> term -> term -> type -> Type :=
 
      | EqSubstAbs :
          forall {G D A B u sbs},
-           issubst sbs G D ->
+           isctx G ->
+           isctx D ->
            istype D A ->
+           istype (ctxextend D A) B ->
            isterm (ctxextend D A) u B ->
+           issubst sbs G D ->
            eqterm G
                   (subst (lam A B u) sbs)
                   (lam
@@ -502,10 +796,13 @@ with eqterm : context -> term -> term -> type -> Type :=
 
      | EqSubstApp :
          forall {G D A B u v sbs},
-           issubst sbs G D ->
+           isctx G ->
+           isctx D ->
+           istype D A ->
            istype (ctxextend D A) B ->
            isterm D u (Prod A B) ->
            isterm D v A ->
+           issubst sbs G D ->
            eqterm G
                   (subst (app u A B v) sbs)
                   (app
@@ -517,8 +814,11 @@ with eqterm : context -> term -> term -> type -> Type :=
 
      | EqSubstRefl :
          forall {G D A u sbs},
-           issubst sbs G D ->
+           isctx G ->
+           isctx D ->
+           istype D A ->
            isterm D u A ->
+           issubst sbs G D ->
            eqterm G
                   (subst (refl A u) sbs)
                   (refl (Subst A sbs) (subst u sbs))
@@ -526,8 +826,10 @@ with eqterm : context -> term -> term -> type -> Type :=
 
      | EqSubstJ :
          forall {G D A C u v w p sbs},
-           issubst sbs G D ->
+           isctx G ->
+           isctx D ->
            istype D A ->
+           issubst sbs G D ->
            isterm D u A ->
            istype
              (ctxextend
@@ -600,11 +902,14 @@ with eqterm : context -> term -> term -> type -> Type :=
                      sbs
                   )
 
+     (* This rule is subsumed by EqTermExfalso *)
      | EqSubstExfalso :
          forall {G D A u sbs},
-           issubst sbs G D ->
+           isctx G ->
+           isctx D ->
            istype D A ->
            isterm D u Empty ->
+           issubst sbs G D ->
            eqterm G
                   (subst (exfalso A u) sbs)
                   (exfalso (Subst A sbs) (subst u sbs))
@@ -612,6 +917,8 @@ with eqterm : context -> term -> term -> type -> Type :=
 
      | EqSubstUnit :
          forall {G D sbs},
+           isctx G ->
+           isctx D ->
            issubst sbs G D ->
            eqterm G
                   (subst unit sbs)
@@ -620,6 +927,8 @@ with eqterm : context -> term -> term -> type -> Type :=
 
      | EqSubstTrue :
          forall {G D sbs},
+           isctx G ->
+           isctx D ->
            issubst sbs G D ->
            eqterm G
                   (subst true sbs)
@@ -628,6 +937,8 @@ with eqterm : context -> term -> term -> type -> Type :=
 
      | EqSubstFalse :
          forall {G D sbs},
+           isctx G ->
+           isctx D ->
            issubst sbs G D ->
            eqterm G
                   (subst false sbs)
@@ -636,6 +947,8 @@ with eqterm : context -> term -> term -> type -> Type :=
 
      | EqSubstCond :
          forall {G D C u v w sbs},
+           isctx G ->
+           isctx D ->
            issubst sbs G D ->
            isterm D u Bool ->
            istype (ctxextend D Bool) C ->
@@ -651,6 +964,7 @@ with eqterm : context -> term -> term -> type -> Type :=
 
      | EqTermExfalso :
          forall {G A u v w},
+           isctx G ->
            istype G A ->
            isterm G u A ->
            isterm G v A ->
@@ -659,18 +973,26 @@ with eqterm : context -> term -> term -> type -> Type :=
 
      | UnitEta :
          forall {G u v},
+           isctx G ->
            isterm G u Unit ->
            isterm G v Unit ->
            eqterm G u v Unit
 
      | EqReflection :
          forall {G A u v w1 w2},
+           isctx G ->
+           istype G A ->
+           isterm G u A ->
+           isterm G v A ->
            isterm G w1 (Id A u v) ->
-           isterm G w2 (UIP A) ->
+           isterm G w2 (reflective A) ->
            eqterm G u v A
 
      | ProdBeta :
          forall {G A B u v},
+           isctx G ->
+           istype G A ->
+           istype (ctxextend G A) B ->
            isterm (ctxextend G A) u B ->
            isterm G v A ->
            eqterm G
@@ -680,6 +1002,7 @@ with eqterm : context -> term -> term -> type -> Type :=
 
      | CondTrue :
          forall {G C v w},
+           isctx G ->
            istype (ctxextend G Bool) C ->
            isterm G v (Subst C (sbzero G Bool true)) ->
            isterm G w (Subst C (sbzero G Bool false)) ->
@@ -690,6 +1013,7 @@ with eqterm : context -> term -> term -> type -> Type :=
 
      | CondFalse :
          forall {G C v w},
+           isctx G ->
            istype (ctxextend G Bool) C ->
            isterm G v (Subst C (sbzero G Bool true)) ->
            isterm G w (Subst C (sbzero G Bool false)) ->
@@ -700,6 +1024,9 @@ with eqterm : context -> term -> term -> type -> Type :=
 
      | ProdEta :
          forall {G A B u v},
+           isctx G ->
+           istype G A ->
+           istype (ctxextend G A) B ->
            isterm G u (Prod A B) ->
            isterm G v (Prod A B) ->
            eqterm (ctxextend G A)
@@ -716,6 +1043,7 @@ with eqterm : context -> term -> term -> type -> Type :=
 
      | JRefl :
          forall {G A C u w},
+           isctx G ->
            istype G A ->
            isterm G u A ->
            istype
@@ -766,6 +1094,13 @@ with eqterm : context -> term -> term -> type -> Type :=
 
      | CongAbs :
          forall {G A1 A2 B1 B2 u1 u2},
+           isctx G ->
+           istype G A1 ->
+           istype G B1 ->
+           istype (ctxextend G A1) A2 ->
+           istype (ctxextend G A1) B2 ->
+           isterm (ctxextend G A1) u1 A2 ->
+           isterm (ctxextend G A1) u2 A2 ->
            eqtype G A1 B1 ->
            eqtype (ctxextend G A1) A2 B2 ->
            eqterm (ctxextend G A1) u1 u2 A2 ->
@@ -776,6 +1111,15 @@ with eqterm : context -> term -> term -> type -> Type :=
 
      | CongApp :
          forall {G A1 A2 B1 B2 u1 u2 v1 v2},
+           isctx G ->
+           istype G A1 ->
+           istype G A2 ->
+           istype (ctxextend G A1) A2 ->
+           istype (ctxextend G A1) B2 ->
+           isterm G u1 (Prod A1 A2) ->
+           isterm G v1 (Prod A1 A2) ->
+           isterm G u2 A1 ->
+           isterm G v2 A1 ->
            eqtype G A1 B1 ->
            eqtype (ctxextend G A1) A2 B2 ->
            eqterm G u1 v1 (Prod A1 A2) ->
@@ -787,6 +1131,11 @@ with eqterm : context -> term -> term -> type -> Type :=
 
      | CongRefl :
          forall {G u1 u2 A1 A2},
+           isctx G ->
+           istype G A1 ->
+           istype G A2 ->
+           isterm G u1 A1 ->
+           isterm G u2 A1 ->
            eqterm G u1 u2 A1 ->
            eqtype G A1 A2 ->
            eqterm G
@@ -796,6 +1145,35 @@ with eqterm : context -> term -> term -> type -> Type :=
 
      | CongJ :
          forall {G A1 A2 C1 C2 u1 u2 v1 v2 w1 w2 p1 p2},
+           isctx G ->
+           istype G A1 ->
+           istype G A2 ->
+           istype
+             (ctxextend
+                (ctxextend G A1)
+                (Id
+                   (Subst A1 (sbweak G A1))
+                   (subst u1 (sbweak G A1))
+                   (var 0)
+                )
+             )
+             C1 ->
+           istype
+             (ctxextend
+                (ctxextend G A1)
+                (Id
+                   (Subst A1 (sbweak G A1))
+                   (subst u1 (sbweak G A1))
+                   (var 0)
+                )
+             )
+             C2 ->
+           isterm G u1 A1 ->
+           isterm G u2 A1 ->
+           isterm G v1 A1 ->
+           isterm G v2 A1 ->
+           isterm G p1 (Id A1 u1 v1) ->
+           isterm G p2 (Id A1 u1 v1) ->
            eqtype G A1 A2 ->
            eqterm G u1 u2 A1 ->
            eqtype
@@ -860,6 +1238,15 @@ with eqterm : context -> term -> term -> type -> Type :=
 
      | CongCond :
          forall {G C1 C2 u1 u2 v1 v2 w1 w2},
+           isctx G ->
+           istype (ctxextend G Bool) C1 ->
+           istype (ctxextend G Bool) C2 ->
+           isterm G u1 Bool ->
+           isterm G u2 Bool ->
+           isterm G v1 (Subst C1 (sbzero G Bool true)) ->
+           isterm G v2 (Subst C1 (sbzero G Bool true)) ->
+           isterm G w1 (Subst C1 (sbzero G Bool false)) ->
+           isterm G w2 (Subst C1 (sbzero G Bool false)) ->
            eqterm G u1 u2 Bool ->
            eqtype (ctxextend G Bool) C1 C2 ->
            eqterm G v1 v2 (Subst C1 (sbzero G Bool true)) ->
@@ -871,6 +1258,11 @@ with eqterm : context -> term -> term -> type -> Type :=
 
      | CongTermSubst :
          forall {G D A u1 u2 sbs},
+           isctx G ->
+           isctx D ->
+           istype D A ->
+           isterm D u1 A ->
+           isterm D u2 A ->
            issubst sbs G D ->
            eqterm D u1 u2 A ->
            eqterm G
@@ -878,52 +1270,563 @@ with eqterm : context -> term -> term -> type -> Type :=
                   (subst u2 sbs)
                   (Subst A sbs).
 
-
-Definition sane_isctx sbs G D :
+Definition sane_issubst sbs G D :
   issubst sbs G D -> isctx G * isctx D.
 Proof.
   intro H ; destruct H.
 
   (* SubstZero *)
   { split.
-    
+
     - assumption.
     - now apply CtxExtend.
   }
 
   (* SubstWeak *)
   { split.
-    
+
     - now apply CtxExtend.
     - assumption.
   }
 
   (* SubstShift *)
   { split.
-    
+
     - apply CtxExtend.
       + assumption.
-      + eapply TySubst.
-        * eassumption.
-        * assumption.
+      + now apply (@TySubst G D).
     - now apply CtxExtend.
   }
 
+  (* SubstId *)
+  { split.
+    - assumption.
+    - assumption.
+  }
+
+  (* SubstComp *)
+  { split.
+    - assumption.
+    - assumption.
+  }
+
+  (* SubstCtxConv *)
+  { split.
+    - assumption.
+    - assumption.
+  }
 Defined.
 
 Definition sane_istype G A :
   istype G A -> isctx G.
 Proof.
+  intro H; destruct H ; assumption.
+Defined.
+
+Definition sane_isterm' G u A :
+  isterm G u A -> istype G A.
+Proof.
+  intro H ; destruct H.
+
+  (* TermTyConv *)
+  { assumption. }
+
+  (* TermCtxConv *)
+  { now apply (@TyCtxConv G D). }
+
+  (* TermSubst *)
+  { now apply (@TySubst G D A sbs). }
+
+  (* TermVarZero *)
+  { eapply TySubst.
+    - now apply (@CtxExtend G A).
+    - eassumption.
+    - now eapply SubstWeak.
+    - assumption.
+  }
+
+  (* TermVarSucc *)
+  { apply (@TySubst (ctxextend G B) G).
+    - now apply CtxExtend.
+    - assumption.
+    - now apply SubstWeak.
+    - assumption.
+  }
+
+  (* TermAbs *)
+  { now apply (@TyProd). }
+
+  (* TermApp *)
+  { apply (@TySubst G (ctxextend G A)).
+    - assumption.
+    - now apply CtxExtend.
+    - now apply SubstZero.
+    - assumption.
+  }
+
+  (* TermRefl *)
+  { now apply TyId. }
+
+  (* TermJ *)
+  { admit. }
+
+  (* TermExfalso *)
+  { assumption. }
+
+  (* TermUnit *)
+  { now apply TyUnit. }
+
+  (* TermTrue *)
+  { now apply TyBool. }
+
+  (* TermFalse *)
+  { now apply TyBool. }
+
+  (* TermCond *)
+  { eapply (@TySubst G (ctxextend G Bool)).
+    + assumption.
+    + apply CtxExtend.
+      * assumption.
+      * now apply TyBool.
+    + apply SubstZero.
+      * assumption.
+      * now apply TyBool.
+      * assumption.
+    + assumption.
+  }
 Admitted.
+
 
 Definition sane_isterm G u A :
   isterm G u A -> isctx G * istype G A.
-Admitted.
+Proof.
+  intro H.
+  pose (K := sane_isterm' G u A H).
+  split ; [now apply (@sane_istype G A) | assumption].
+Defined.
 
-Definition sane_eqtype G A B :
+Definition sane_eqtype' G A B :
+  eqtype G A B -> istype G A * istype G B.
+Proof.
+  intro H ; destruct H.
+
+  (* EqTyCtxConv *)
+  { split.
+    - { now apply (@TyCtxConv G D). }
+    - { now apply (@TyCtxConv G D). }
+  }
+
+  (* EqTyRefl*)
+  { split ; assumption. }
+
+  (* EqTySym *)
+  { split ; assumption. }
+
+  (* EqTyTrans *)
+  { split ; assumption. }
+
+  (* EqTyIdSubst *)
+  { split.
+    - eapply TySubst.
+      + assumption.
+      + eassumption.
+      + now apply SubstId.
+      + assumption.
+    - assumption.
+  }
+
+  (* EqTySubstComp *)
+  { split.
+    - apply (@TySubst G D) ; auto.
+      apply (@TySubst D E) ; auto.
+    - apply (@TySubst G E) ; auto.
+      apply (@SubstComp G D E) ; auto.
+  }
+
+  (* EqTySubstProd *)
+  { split.
+    - { apply (@TySubst G D) ; auto using TyProd. }
+    - { apply TyProd ; auto.
+        + now apply (@TySubst G D).
+        + apply (@TySubst _ (ctxextend D A)) ; auto.
+          * apply CtxExtend ; auto.
+            now apply (@TySubst G D).
+          * now apply CtxExtend.
+          * now apply SubstShift.
+      }
+  }
+
+  (* EqTySubstId *)
+  { split.
+    - { apply (@TySubst G D) ; auto using TyId. }
+    - { apply TyId ; auto using (@TySubst G D), (@TermSubst G D). }
+  }
+
+  (* EqTySubstEmpty *)
+  { split.
+    - { apply (@TySubst G D) ; auto using TyEmpty. }
+    - { now apply TyEmpty. }
+  }
+
+  (* EqTySubstUnit *)
+  { split.
+    - { apply (@TySubst G D) ; auto using TyUnit. }
+    - { now apply TyUnit. }
+  }
+
+  (* EqTySubstBool *)
+  { split.
+    - { apply (@TySubst G D) ; auto using TyBool. }
+    - { now apply TyBool. }
+  }
+
+  (* EqTyExfalso *)
+  { split ; assumption. }
+
+  (* CongProd *)
+  { split.
+    - { now apply TyProd. }
+    - { apply TyProd ; auto.
+        apply (@TyCtxConv (ctxextend G A1)) ; auto using CtxExtend.
+        now apply EqCtxExtend. }
+      }
+
+  (* CongId *)
+  { split.
+    - { now apply TyId. }
+    - { apply TyId.
+        - assumption.
+        - assumption.
+        - now apply (@TermTyConv G A B v1).
+        - now apply (@TermTyConv G A B v2).
+      }
+  }
+
+  (* CongTySubst *)
+  { split.
+    - { now apply (@TySubst G D). }
+    - { now apply (@TySubst G D). }
+  }
+
+Defined.
+
+Theorem sane_eqctx G D :
+  eqctx G D -> isctx G * isctx D.
+Proof.
+  intro H ; destruct H.
+
+  (* CtxRefl *)
+  { split.
+    - assumption.
+    - assumption.
+  }
+
+  (* CtxSym *)
+  { split.
+    - assumption.
+    - assumption.
+  }
+
+  (* CtxTrans *)
+  { split.
+    - assumption.
+    - assumption.
+  }
+
+  (* EqCtxEmpty *)
+  { split.
+    - now apply CtxEmpty.
+    - now apply CtxEmpty.
+  }
+
+  (* EqCtxExtend *)
+  { split.
+    - now apply CtxExtend.
+    - now apply CtxExtend.
+  }
+
+Defined.
+
+Theorem sane_eqtype G A B :
   eqtype G A B -> isctx G * istype G A * istype G B.
-Admitted.
+Proof.
+  intro H.
+  destruct (sane_eqtype' G A B H).
+  auto using (sane_istype G A).
+Defined.
 
-Definition isctx_from_eqterm G u v A :
-  eqterm G u v A -> isctx G * istype G A * isterm G u A * isterm G v A.
+Theorem sane_eqterm' G u v A :
+  eqterm G u v A -> isterm G u A * isterm G v A.
+Proof.
+  intro H ; destruct H.
+
+  (* EqTyConv *)
+  - { split.
+      - { now apply (@TermTyConv G A B u). }
+      - { now apply (@TermTyConv G A B v). }
+    }
+
+  (* EqCtxConv *)
+  - { split.
+      - { now apply (@TermCtxConv G D A). }
+      - { now apply (@TermCtxConv G D A). }
+    }
+
+  (* EqRefl *)
+  - { split.
+      - { assumption. }
+      - { assumption. }
+    }
+
+  (* EqSym *)
+  - { split.
+      - { assumption. }
+      - { assumption. }
+    }
+
+  (* EqTrans *)
+  - { split.
+      - { assumption. }
+      - { assumption. }
+    }
+
+  (* EqIdSubst *)
+  - { split.
+      - { apply (@TermTyConv G (Subst A (sbid G)) A).
+          - assumption.
+          - apply (@TySubst G G) ; auto using SubstId.
+          - assumption.
+          - apply (@TermSubst G G) ; auto using SubstId.
+          - now apply EqTyIdSubst.
+        }
+      - { assumption. }
+    }
+
+  (* EqSubstComp *)
+  - { split.
+      - { apply (@TermTyConv G (Subst (Subst A sbt) sbs) (Subst A (sbcomp sbt sbs))).
+          - assumption.
+          - apply (@TySubst G D) ; auto.
+            now apply (@TySubst D E).
+          - apply (@TySubst G E) ; auto.
+            now apply (@SubstComp G D E).
+          - apply (@TermSubst G D) ; auto.
+            + now apply (@TySubst D E).
+            + now apply (@TermSubst D E).
+          - now apply (@EqTySubstComp G D E).
+        }
+      - { apply (@TermSubst G E) ; auto.
+          now apply (@SubstComp G D E).
+        }
+    }
+
+  (* EqSubstWeak *)
+  - { split.
+      - { apply (@TermSubst _ G) ; auto using CtxExtend.
+          now apply SubstWeak.
+        }
+      - { now apply TermVarSucc. }
+    }
+
+
+  (* EqSubstZeroZero *)
+  - { split.
+      - { apply (@TermTyConv G (Subst (Subst A (sbweak G A)) (sbzero G A u))).
+          - assumption.
+          - apply (@TySubst _ (ctxextend G A)) ; auto using CtxExtend.
+            + now apply SubstZero.
+            + apply (@TySubst _ G) ; auto using CtxExtend.
+              now apply SubstWeak.
+          - assumption.
+          - apply (@TermSubst _ (ctxextend G A)) ; auto using CtxExtend.
+            + apply (@TySubst _ G) ; auto using CtxExtend, SubstWeak.
+            + now apply SubstZero.
+            + now apply TermVarZero.
+          - apply (@EqTyTrans G _ (Subst A (sbid G))) ; auto.
+            + apply (@TySubst _ (ctxextend G A)) ; auto using CtxExtend.
+              * now apply SubstZero.
+              * apply (@TySubst _ G) ; auto using CtxExtend, SubstWeak.
+            + apply (@TySubst _ G) ; auto using SubstId.
+            + { apply (@EqTyTrans _ _ (Subst A (sbcomp (sbweak G A) (sbzero G A u)))) ; auto.
+                - apply (@TySubst _ (ctxextend G A)) ; auto using CtxExtend, SubstZero.
+                  apply (@TySubst _ G) ; auto using CtxExtend, SubstWeak.
+                - apply (@TySubst _ G) ; auto.
+                  + apply (@SubstComp _ (ctxextend G A)) ; auto using CtxExtend, SubstWeak, SubstZero.
+                - apply (@TySubst _ G) ; auto using SubstId.
+                - apply (@EqTySubstComp G (ctxextend G A) G) ;
+                  auto using CtxExtend, (@SubstComp G (ctxextend G A)) , SubstWeak, SubstZero.
+                - apply (@CongTySubst G G) ;
+                  auto using CtxExtend, (@SubstComp G (ctxextend G A)) , SubstWeak, SubstZero, SubstId, EqTyRefl.
+              }
+            + now apply EqTyIdSubst.
+        }
+      - { assumption. }
+    }
+
+  (* EqSubstZeroSucc *)
+  - { split.
+      - { apply (@TermTyConv G (Subst (Subst A (sbweak G B)) (sbzero G B u))).
+          - assumption.
+          - apply (@TySubst _ (ctxextend G B)) ; auto using CtxExtend, SubstZero.
+            apply (@TySubst _ G) ; auto using CtxExtend, SubstWeak.
+          - assumption.
+          - apply (@TermSubst G (ctxextend G B)) ; auto using CtxExtend.
+            + apply (@TySubst _ G) ; auto using CtxExtend, SubstWeak.
+            + now apply SubstZero.
+            + now apply TermVarSucc.
+          - admit.
+        }
+      - { assumption. }
+    }
+
+  (* EqSubstShiftZero *)
+  - { split.
+      - { admit. }
+      - { admit. }
+    }
+
+  (* EqSubstShiftSucc *)
+  - { split.
+      - { admit. }
+      - { admit. }
+    }
+
+  (* EqSubstAbs *)
+  - { split.
+      - { admit. }
+      - { admit. }
+    }
+
+  (* EqSubstApp *)
+  - { split.
+      - { admit. }
+      - { admit. }
+    }
+
+  (* EqSubstRefl *)
+  - { split.
+      - { admit. }
+      - { admit. }
+    }
+
+  (* EqSubstJ *)
+  - { split.
+      - { admit. }
+      - { admit. }
+    }
+
+  (* EqSubstExfalso *)
+  - { split.
+      - { admit. }
+      - { admit. }
+    }
+
+  (* EqSubstUnit *)
+  - { split.
+      - { admit. }
+      - { admit. }
+    }
+
+  (* EqSubstTrue *)
+  - { split.
+      - { admit. }
+      - { admit. }
+    }
+
+  (* EqSubstFalse *)
+  - { split.
+      - { admit. }
+      - { admit. }
+    }
+
+  (* EqSubstCond *)
+  - { split.
+      - { admit. }
+      - { admit. }
+    }
+
+  (* EqTermExfalso *)
+  - { split.
+      - { admit. }
+      - { admit. }
+    }
+
+  (* UnitEta *)
+  - { split.
+      - { admit. }
+      - { admit. }
+    }
+
+  (* EqReflection *)
+  - { split.
+      - { admit. }
+      - { admit. }
+    }
+
+  (* ProdBeta *)
+  - { split.
+      - { admit. }
+      - { admit. }
+    }
+
+  (* CondTrue *)
+  - { split.
+      - { admit. }
+      - { admit. }
+    }
+
+  (* CondFalse *)
+  - { split.
+      - { admit. }
+      - { admit. }
+    }
+
+  (* ProdEta *)
+  - { split.
+      - { admit. }
+      - { admit. }
+    }
+
+  (* JRefl *)
+  - { split.
+      - { admit. }
+      - { admit. }
+    }
+
+  (* CongAbs *)
+  - { split.
+      - { admit. }
+      - { admit. }
+    }
+
+  (* CongApp *)
+  - { split.
+      - { admit. }
+      - { admit. }
+    }
+
+  (* CongRefl *)
+  - { split.
+      - { admit. }
+      - { admit. }
+    }
+
+  (* CongJ *)
+  - { split.
+      - { admit. }
+      - { admit. }
+    }
+
+  (* CongCond *)
+  - { split.
+      - { admit. }
+      - { admit. }
+    }
+
+  (* CongTermSubst *)
+  - { split.
+      - { admit. }
+      - { admit. }
+    }
+
 Admitted.
