formalization/paranoidSanity.v
@@ -1,0 +1,181 @@
+Require Import syntax.
+Require ett ptt.
+
+Axiom postpone_proof : forall A : Type, A.
+Ltac later := apply postpone_proof.
+
+Fixpoint sane_isctx G (P : ett.isctx G) {struct P} : ptt.isctx G
+
+with sane_issubst sbs G D (P : ett.issubst sbs G D) {struct P} : ptt.issubst sbs G D
+
+with sane_istype G A (P : ett.istype G A) {struct P} : ptt.istype G A
+
+with sane_isterm G u A (P : ett.isterm G u A) {struct P} : ptt.isterm G u A
+
+with sane_eqsubst sbs sbt G D (P : ett.eqsubst sbs sbt G D) {struct P} : ptt.eqsubst sbs sbt G D
+
+with sane_eqctx G D (P : ett.eqctx G D) {struct P} : ptt.eqctx G D
+
+with sane_eqtype G A B (P : ett.eqtype G A B) {struct P} : ptt.eqtype G A B
+
+with sane_eqterm G u v A (P : ett.eqterm G u v A) {struct P} : ptt.eqterm G u v A.
+
+Proof.
+
+  (* sane_isctx *)
+  { destruct P.
+
+    (* CtxEmpty *)
+    - { apply ptt.CtxEmpty. }
+
+    (* CtxExtend *)
+    - {
+        intros ; apply ptt.CtxExtend.
+        + now apply sane_isctx.
+        + now apply sane_istype.
+      }
+  }
+
+  (* sane_issubst *)
+  { destruct P.
+
+    (* SubstZero *)
+    - { apply ptt.SubstZero.
+        + eapply ptt.sane_isterm.
+          eapply sane_isterm ; eassumption.
+        + eapply ptt.sane_isterm.
+          eapply sane_isterm ; eassumption.
+        + now apply sane_isterm.
+      }
+
+    (* SubstWeak *)
+    - {
+        apply ptt.SubstWeak.
+        + eapply ptt.sane_istype.
+          eapply sane_istype ; eassumption.
+        + now apply sane_istype.
+      }
+
+    (* SubstShift. *)
+    - {
+        apply ptt.SubstShift.
+        + eapply (ptt.sane_issubst sbs G D).
+          now apply sane_issubst.
+        + eapply (ptt.sane_istype D A).
+          now apply sane_istype.
+        + now apply sane_issubst.
+        + now apply sane_istype.
+      }
+
+     (* SubstId *)
+     - {
+         apply ptt.SubstId.
+         - now apply sane_isctx.
+       }
+
+     (* SubstComp *)
+     - {
+         apply (@ptt.SubstComp G D E).
+         - apply (ptt.sane_issubst sbs G D).
+           now apply sane_issubst.
+         - apply (ptt.sane_issubst sbt D E).
+           now apply sane_issubst.
+         - apply (ptt.sane_issubst sbt D E).
+           now apply sane_issubst.
+         - now apply sane_issubst.
+         - now apply sane_issubst.
+       }
+
+     (* SubstCtxConv *)
+     - {
+         apply (@ptt.SubstCtxConv G1 G2 D1 D2).
+         - apply (ptt.sane_eqctx G1 G2).
+           now apply sane_eqctx.
+         - apply (ptt.sane_eqctx G1 G2).
+           now apply sane_eqctx.
+         - apply (ptt.sane_eqctx D1 D2).
+           now apply sane_eqctx.
+         - apply (ptt.sane_eqctx D1 D2).
+           now apply sane_eqctx.
+         - now apply sane_issubst.
+         - now apply sane_eqctx.
+         - now apply sane_eqctx.
+       }
+  }
+
+  (* sane_istype *)
+  { destruct P.
+
+    (* TyCtxConv *)
+    { apply (@ptt.TyCtxConv G D).
+      - now apply (ptt.sane_eqctx G D), sane_eqctx.
+      - now apply (ptt.sane_eqctx G D), sane_eqctx.
+      - now apply sane_istype.
+      - now apply sane_eqctx.
+    }
+
+    (* TySubst *)
+    { apply (@ptt.TySubst G D).
+      - now apply (ptt.sane_issubst sbs G D), sane_issubst.
+      - now apply (ptt.sane_istype D A), sane_istype.
+      - now apply sane_issubst.
+      - now apply sane_istype.
+    }
+
+    (* TyProd *)
+    { apply ptt.TyProd.
+      - now apply (ptt.sane_istype G A), sane_istype.
+      - now apply sane_istype.
+      - now apply sane_istype.
+    }
+
+    (* TyId *)
+    { apply ptt.TyId.
+      - now apply (ptt.sane_istype G A), sane_istype.
+      - now apply sane_istype.
+      - now apply sane_isterm.
+      - now apply sane_isterm.
+    }
+
+    (* TyEmpty *)
+    { apply ptt.TyEmpty.
+      - now apply sane_isctx.
+    }
+
+    (* TyUnit *)
+    { apply ptt.TyUnit.
+      - now apply sane_isctx.
+    }
+
+    (* TyBool *)
+    { apply ptt.TyBool.
+      - now apply sane_isctx.
+    }
+  }
+
+  (* sane_isterm *)
+  {
+    later.
+  }
+
+  (* sane_eqsubst *)
+  {
+    later.
+  }
+
+  (* sane_eqctx *)
+  {
+    later.
+  }
+
+  (* sane_eqtype *)
+  {
+    later.
+  }
+
+  (* sane_eqterm *)
+  {
+    later.
+  }
+
+Defined.
